@prefix rdf: <http://www.w3.org/1999/02/22-rdf-syntax-ns#> .
@prefix rdfs: <http://www.w3.org/2000/01/rdf-schema#> .
@prefix qb: <http://purl.org/linked-data/cube#> .
@prefix owl: <http://www.w3.org/2002/07/owl#> .
@prefix hobbit: <http://w3id.org/hobbit/vocab#> .
@prefix xsd: <http://www.w3.org/2001/XMLSchema#> .
@prefix mexcore: <http://mex.aksw.org/mex-core#> .

# --- Resources ---

hobbit:AscendingOrder
  rdf:type hobbit:Ranking ;
  rdfs:comment "Indicates smallest-to-largest preferred ordering of property values."^^xsd:string ;
  rdfs:label "Ascending Order"^^xsd:string .

hobbit:DescendingOrder
  rdf:type hobbit:Ranking ;
  rdfs:comment "Indicates largest-to-smallest preferred ordering of property values."^^xsd:string ;
  rdfs:label "Descending Order"^^xsd:string .

hobbit:PearsonAlgorithm a hobbit:AnalysisAlgorithm ;
  rdf:type hobbit:AnalysisAlgorithm ;
  rdfs:label "Pearson"@en ;
  rdfs:comment "Pearson correlation coefficient."@en .

# --- Classes ---

hobbit:AnalysisAlgorithm
  rdf:type owl:Class ;
  rdfs:comment "Instances of this class define algorithms which compute correlation."^^xsd:string ;
  rdfs:label "Analysis Algorithm"^^xsd:string .

hobbit:AnalysisResult
  rdf:type owl:Class ;
  rdfs:comment "Instances of this class define correlation data for a pair of hobbit:Parameter and hobbit:KPI in a hobbit:AnalysisResultset."^^xsd:string ;
  rdfs:label "Analysis Result"^^xsd:string .

hobbit:AnalysisResultset
  rdf:type owl:Class ;
  rdfs:comment "Instances of this class define a resultset of correlation data for a pair of hobbit:Benchmark and hobbit:System."^^xsd:string ;
  rdfs:label "Analysis Resultset"^^xsd:string .

hobbit:Benchmark
  rdf:type owl:Class;
  rdfs:comment "Instances of this class define a particular benchmark."^^xsd:string ;
  rdfs:label "Benchmark"^^xsd:string .

hobbit:Challenge
  rdf:type owl:Class;
  rdfs:comment "Instances of this class define a challenge with its single   hobbit:ChallengeTasks."^^xsd:string ;
  rdfs:label "Challenge"^^xsd:string .

hobbit:ChallengeTask
  rdf:type owl:Class;
  rdfs:comment "A challenge task is a part of a challenge that involves a benchmark with a   certain parameterization and a list of systems."^^xsd:string ;
  rdfs:label "Challenge Task"^^xsd:string .

hobbit:Ranking
  rdf:type owl:Class ;
  rdfs:comment "Instances of this class define an ordering of property values."^^xsd:string ;
  rdfs:label "Ranking"^^xsd:string .

hobbit:KPISeq
  rdf:type owl:Class ;
  owl:equivalentClass [
    a owl:Class ;
    owl:intersectionOf (
      rdf:Seq
      [
        a owl:Restriction ;
        owl:onProperty rdf:li ;
        owl:allValuesFrom hobbit:KPI
      ]
    )
  ] ;
  rdfs:comment "RDF Sequence of KPI resources."^^xsd:string ;
  rdfs:label "KPI Sequence"^^xsd:string .


hobbit:SystemInstance
  rdf:type owl:Class;
  rdfs:comment "Instances of a system that can be mapped to a docker image."^^xsd:string ;
  rdfs:label "System Instance"^^xsd:string .

hobbit:System
  rdf:type owl:Class;
  rdfs:comment "Express the connection between single system instances that represent different configurations of the same system. "^^xsd:string ;
  rdfs:label "System"^^xsd:string .

hobbit:API
  rdf:type owl:Class;
  rdfs:comment "Connects the benchmark with the API the benchmarked system will have to implement to be benchmarked."^^xsd:string ;
  rdfs:label "API"^^xsd:string .

hobbit:Hardware
  rdf:type owl:Class;
  rdfs:comment "Hardware setup on which the experiment has been carried out on."^^xsd:string ;
  rdfs:label "Hardware setup"^^xsd:string .

hobbit:Experiment
  rdf:type owl:Class;
  rdfs:comment "Description of an experiment"^^xsd:string ;
  rdfs:label "Experiment"^^xsd:string ;
  rdfs:domain hobbit:KPI .

hobbit:Error
  rdf:type owl:Class;
  rdfs:comment "Why an experiment didnâ€™t terminated in a healthy state"^^xsd:string ;
  rdfs:label "Error"^^xsd:string .


# --- Properties ---

hobbit:Parameter
  rdfs:subClassOf rdf:Property;
  rdfs:comment "Instances of this class define a parameter property with a label, a description and a value type (using a range definition). "^^xsd:string ;
  rdfs:label "Parameter"^^xsd:string ;
  rdfs:range xsd:string ;
  rdfs:domain [ owl:unionOf (hobbit:SystemInstance hobbit:Experiment) ] .

hobbit:ConfigurableParameter
  rdfs:subClassOf hobbit:Parameter ;
  rdfs:comment " An instance of hobbit:Experiment class involving a benchmark that has defined these parameters should use the instances to define the values of the parameters."^^xsd:string ;
  rdfs:label "Configurable Parameter"^^xsd:string .

hobbit:FeatureParameter
  rdfs:subClassOf hobbit:Parameter ;
  rdfs:subClassOf qb:DimensionProperty ;
  rdfs:comment "Instances of this class define a parameter that can be used as features of a system or a benchmark during later analysis. Instances of this class can be created at runtime."^^xsd:string ;
  rdfs:label "Feature Parameter"^^xsd:string .

hobbit:ForwardedParameter
  rdfs:subClassOf hobbit:Parameter ;
  rdfs:subClassOf qb:DimensionProperty ;
  rdfs:comment "Instances of this class define a parameter that can be part of a benchmark configuration and will be forwarded to the system by the platform."^^xsd:string ;
  rdfs:label "Forwarded Parameter"^^xsd:string .

hobbit:KPI
  rdfs:subClassOf rdf:Property ;
  rdfs:subClassOf qb:MeasureProperty ;
  rdfs:comment "Instances of this class define a measure property."^^xsd:string ;
  rdfs:label "KPI"^^xsd:string ;
  rdfs:domain hobbit:Experiment ;
  rdfs:range xsd:string .

# --- Datatype Properties ---

hobbit:imageName
  rdfs:subPropertyOf hobbit:usesImage ;
  rdfs:comment "The docker image name of a hobbit:Benchmark or a hobbit:SystemInstance."^^xsd:string ;
  rdfs:label "Docker Image Name"^^xsd:string ;
  rdfs:domain [ owl:unionOf (hobbit:SystemInstance  hobbit:Benchmark) ] ;
  rdfs:range xsd:string .

hobbit:usesImage
  rdf:type owl:DatatypeProperty ;
  rdfs:comment "The name of a docker image used by this hobbit:Benchmark or hobbit:SystemInstance."^^xsd:string ;
  rdfs:label "Makes use of this Docker image"^^xsd:string ;
  rdfs:domain [ owl:unionOf (hobbit:SystemInstance  hobbit:Benchmark) ] ;
  rdfs:range xsd:string .

hobbit:version
  rdf:type owl:DatatypeProperty ;
  rdfs:comment "The version of the benchmark."^^xsd:string ;
  rdfs:label "Benchmark Version"^^xsd:string ;
  rdfs:domain hobbit:Benchmark ;
  rdfs:range xsd:string .

hobbit:executionDate
  rdf:type owl:DatatypeProperty ;
  rdfs:comment "The date at which the execution of the experiments of a challenge starts."^^xsd:string ;
  rdfs:label "Execution Date"^^xsd:string ;
  rdfs:domain hobbit:Challenge ;
  rdfs:range xsd:date .

hobbit:publicationDate
  rdf:type owl:DatatypeProperty ;
  rdfs:comment "The data at which the challenge results will be copied into the public graph, i.e., be publicly available."^^xsd:string ;
  rdfs:label "Publication Date"^^xsd:string ;
  rdfs:domain hobbit:Challenge ;
  rdfs:range xsd:date .

hobbit:organizer
  rdf:type owl:DatatypeProperty ;
  rdfs:comment "The user identifier of the challenge organizer."^^xsd:string ;
  rdfs:label "Organizer"^^xsd:string ;
  rdfs:domain hobbit:Challenge ;
  rdfs:range xsd:string .

hobbit:registrationCutoffDate
  rdf:type owl:DatatypeProperty ;
  rdfs:comment "Date after which no more systems can be registered for a challenge."^^xsd:string ;
  rdfs:label "Registration Cutoff Date"^^xsd:string ;
  rdfs:domain hobbit:Challenge ;
  rdfs:range xsd:dateTime .

hobbit:executionPeriod
  rdf:type owl:DatatypeProperty ;
  rdfs:comment "Time between consecutive executions."^^xsd:string ;
  rdfs:label "Period"^^xsd:string ;
  rdfs:domain hobbit:Challenge ;
  rdfs:range xsd:string .

hobbit:dateOfNextExecution
  rdf:type owl:DatatypeProperty ;
  rdfs:comment "Date at which the execution takes place next time."^^xsd:string ;
  rdfs:label "Date of Next Execution"^^xsd:string ;
  rdfs:domain hobbit:Challenge ;
  rdfs:range xsd:dateTime .

hobbit:visible
  rdf:type owl:DatatypeProperty ;
  rdfs:comment "A flag indicating whether a hobbit:Challenge is visible to the public."^^xsd:string ;
  rdfs:label "Visibility"^^xsd:string ;
  rdfs:domain hobbit:Challenge ;
  rdfs:range xsd:boolean .

hobbit:startTime
  rdf:type owl:DatatypeProperty ;
  rdfs:comment "The timestamp of the start of the hobbit:Experiment."^^xsd:string ;
  rdfs:label "Start Time"^^xsd:string ;
  rdfs:domain hobbit:Experiment ;
  rdfs:range xsd:dateTime .

hobbit:endTime
  rdf:type owl:DatatypeProperty ;
  rdfs:comment "The timestamp of the end of a hobbit:Experiment."^^xsd:string ;
  rdfs:label "End Time"^^xsd:string ;
  rdfs:domain hobbit:Experiment ;
  rdfs:range xsd:dateTime .

hobbit:hobbitPlatformVersion
  rdf:type owl:DatatypeProperty ;
  rdfs:comment "The version of the HOBBIT platform that has been used to carry out the experiment."^^xsd:string ;
  rdfs:label "Platform Version"^^xsd:string ;
  rdfs:domain hobbit:Experiment ;
  rdfs:range xsd:string .

hobbit:defaultValue
  rdf:type owl:DatatypeProperty ;
  rdfs:comment "A default value of a hobbit:Parameter."^^xsd:string ;
  rdfs:label "Deafult Value"^^xsd:string ;
  rdfs:domain hobbit:ConfigurableParameter ;
  rdfs:range xsd:string .

hobbit:relevantForAnalysis
  rdf:type owl:DatatypeProperty ;
  rdfs:comment "A flag indicating whether a hobbit:Parameter should be used by the analysis component (default) or it should be ignored."^^xsd:string ;
  rdfs:label "Relevant for Analysis"^^xsd:string ;
  rdfs:domain hobbit:Parameter ;
  rdfs:range xsd:boolean .

hobbit:hasModel
  rdf:type owl:DatatypeProperty ;
  rdfs:comment ""^^xsd:string ;
  rdfs:label ""^^xsd:string ;
  rdfs:domain hobbit:Hardware ;
  rdfs:range xsd:string .

hobbit:hasProcessors
  rdf:type owl:DatatypeProperty ;
  rdfs:comment ""^^xsd:string ;
  rdfs:label ""^^xsd:string ;
  rdfs:domain hobbit:Hardware ;
  rdfs:range xsd:string .

hobbit:hasMemory
  rdf:type owl:DatatypeProperty ;
  rdfs:comment ""^^xsd:string ;
  rdfs:label ""^^xsd:string ;
  rdfs:domain hobbit:Hardware ;
  rdfs:range xsd:string .


hobbit:hasDisks
  rdf:type owl:DatatypeProperty ;
  rdfs:comment ""^^xsd:string ;
  rdfs:label ""^^xsd:string ;
  rdfs:domain hobbit:Hardware ;
  rdfs:range xsd:string .

hobbit:hasNetworkAdapters
  rdf:type owl:DatatypeProperty ;
  rdfs:comment ""^^xsd:string ;
  rdfs:label ""^^xsd:string ;
  rdfs:domain hobbit:Hardware ;
  rdfs:range xsd:string .

hobbit:hasOS
  rdf:type owl:DatatypeProperty ;
  rdfs:comment ""^^xsd:string ;
  rdfs:label ""^^xsd:string ;
  rdfs:domain hobbit:Hardware ;
  rdfs:range xsd:string .

hobbit:hasFileSystem
  rdf:type owl:DatatypeProperty ;
  rdfs:comment ""^^xsd:string ;
  rdfs:label ""^^xsd:string ;
  rdfs:domain hobbit:Hardware ;
  rdfs:range xsd:string .

hobbit:hasCPUTypeCount
  rdf:type owl:DatatypeProperty ;
  rdfs:comment ""^^xsd:string ;
  rdfs:label ""^^xsd:string ;
  rdfs:domain hobbit:Hardware ;
  rdfs:range xsd:string .

hobbit:hasRAM
  rdf:type owl:DatatypeProperty ;
  rdfs:comment ""^^xsd:string ;
  rdfs:label ""^^xsd:string ;
  rdfs:domain hobbit:Hardware ;
  rdfs:range xsd:string .

hobbit:closed
  rdf:type owl:DatatypeProperty ;
  rdfs:comment "A flag indicating whether a hobbit:Challenge is closed/finalized and no more changes are allowed "^^xsd:string ;
  rdfs:label "Challenge Flag"^^xsd:string ;
  rdfs:domain hobbit:Challenge ;
  rdfs:range xsd:boolean .

# --- Object Properties ---

hobbit:algorithm
  rdf:type owl:ObjectProperty ;
  rdfs:comment "Analysis result was computed using this algorithm."^^xsd:string ;
  rdfs:label "Algorithm used"^^xsd:string ;
  rdfs:domain hobbit:AnalysisResult ;
  rdfs:range hobbit:AnalysisAlgorithm .

hobbit:measuresKPI
  rdf:type owl:ObjectProperty ;
  rdfs:comment "The hobbit:benchmark measures the KPI and will return it as result "^^xsd:string ;
  rdfs:label "KPI result"^^xsd:string ;
  rdfs:domain hobbit:Benchmark ;
  rdfs:range hobbit:KPI .

hobbit:hasAPI
  rdf:type owl:ObjectProperty ;
  rdfs:comment "Connects the benchmark with the API the benchmarked system will have to implement to be benchmarked."^^xsd:string ;
  rdfs:label "Has API"^^xsd:string ;
  rdfs:domain hobbit:Benchmark ;
  rdfs:range hobbit:API .

hobbit:hasParameter
  rdf:type owl:ObjectProperty ;
  rdfs:comment "Connects the benchmark to the parameters with which the benchmark can be configured."^^xsd:string ;
  rdfs:label "Has Parameter"^^xsd:string ;
  rdfs:domain hobbit:Benchmark ;
  rdfs:range hobbit:Parameter .

hobbit:involvesBenchmark
  rdf:type owl:ObjectProperty ;
  rdfs:comment "Connects the hobbit:experiment or hobbit:ChallengeTask to the hobbit:Benchmark instance that has been used for the experiment.."^^xsd:string ;
  rdfs:label "Involved Benchmark"^^xsd:string ;
  rdfs:domain [owl:unionOf (hobbit:Experiment hobbit:ChallengeTask hobbit:AnalysisResultset)] ;
  rdfs:range hobbit:Benchmark .

hobbit:involvesKPI
  rdf:type owl:ObjectProperty ;
  rdfs:comment "Connects the hobbit:AnalysisResult to the hobbit:KPI that has been used to compute correlation."^^xsd:string ;
  rdfs:label "Involved KPI"^^xsd:string ;
  rdfs:domain hobbit:AnalysisResult ;
  rdfs:range hobbit:KPI .

hobbit:involvesParameter
  rdf:type owl:ObjectProperty ;
  rdfs:comment "Connects the hobbit:AnalysisResult to the hobbit:Parameter that has been used to compute correlation."^^xsd:string ;
  rdfs:label "Involved Parameter"^^xsd:string ;
  rdfs:domain hobbit:AnalysisResult ;
  rdfs:range hobbit:Parameter .

hobbit:involvesSystemInstance
  rdf:type owl:ObjectProperty ;
  rdfs:comment "Connects the hobbit:experiment or hobbit:ChallengeTask to the hobbit:SystemInstance that has been benchmarked in this experiment."^^xsd:string ;
  rdfs:label "Involved System Instance"^^xsd:string ;
  rdfs:domain [owl:unionOf (hobbit:Experiment hobbit:ChallengeTask hobbit:AnalysisResultset)] ;
  rdfs:range hobbit:SystemInstance .

hobbit:isTaskOf
  rdf:type owl:ObjectProperty ;
  rdfs:comment "Connects hobbit:ChallengeTask to a hobbit:Challenge."^^xsd:string ;
  rdfs:label "Part of"^^xsd:string ;
  rdfs:domain hobbit:ChallengeTask ;
  rdfs:range hobbit:Challenge .

hobbit:isPartOf
  rdf:type owl:ObjectProperty ;
  rdfs:comment "Connects the hobbit:experiment to a hobbit:ChallengeTask."^^xsd:string ;
  rdfs:label "Part of"^^xsd:string ;
  rdfs:domain hobbit:Experiment ;
  rdfs:range hobbit:ChallengeTask .

hobbit:implementsAPI
  rdf:type owl:ObjectProperty ;
  rdfs:comment "Connects the hobbit:SystemInstance with the API it implements."^^xsd:string ;
  rdfs:label "Implements API"^^xsd:string ;
  rdfs:domain hobbit:SystemInstance ;
  rdfs:range hobbit:API .

hobbit:instanceOf
  rdf:type owl:ObjectProperty ;
  rdfs:comment "Connects the hobbit:SystemInstance to the hobbit:System of which it is a configured instance."^^xsd:string ;
  rdfs:label "Instance Of"^^xsd:string ;
  rdfs:domain hobbit:SystemInstance ;
  rdfs:range hobbit:System .

hobbit:hasParameter
  rdf:type owl:ObjectProperty ;
  rdfs:comment "Connects the hobbit:Benchmark to the hobbit:Parameter with which the benchmark can be configured."^^xsd:string ;
  rdfs:label "Has Parameter"^^xsd:string ;
  rdfs:domain hobbit:System ;
  rdfs:range hobbit:Parameter .

hobbit:wasCarriedOutOn
  rdf:type owl:ObjectProperty ;
  rdfs:comment "Connects the hobbit:Experiment to the description of hardware that has been used to carry out the experiment."^^xsd:string ;
  rdfs:label "Hardware setup specifications"^^xsd:string ;
  rdfs:domain hobbit:Experiment ;
  rdfs:range hobbit:Hardware .

hobbit:comprises
  rdf:type owl:ObjectProperty ;
  rdfs:comment "Connects the hardware setup description to the hardware node description."^^xsd:string ;
  rdfs:label "Hardware node specifications"^^xsd:string ;
  rdfs:domain hobbit:Hardware ;
  rdfs:range mexcore:HardwareConfiguration .

hobbit:terminatedWithError
  rdf:type owl:ObjectProperty ;
  rdfs:comment "Connects the hobbit:Experiment to the error, if an error occurred"^^xsd:string ;
  rdfs:label "Error of the experiment"^^xsd:string ;
  rdfs:domain hobbit:Experiment ;
  rdfs:range hobbit:Error .

hobbit:ranking
  rdf:type owl:ObjectProperty ;
  rdfs:comment "Connects the hobbit:KPI to one of hobbit:Ranking resources which indicates the preferred ordering of KPI values."^^xsd:string ;
  rdfs:label "Ranking of KPI"^^xsd:string ;
  rdfs:domain hobbit:KPI ;
  rdfs:range hobbit:Ranking .

hobbit:rankingKPIs
  rdf:type owl:ObjectProperty ;
  rdfs:comment "List of KPIs used for ordering Systems by rank."^^xsd:string ;
  rdfs:label "Ranking KPIs"^^xsd:string ;
  rdfs:domain hobbit:ChallengeTask ;
  rdfs:range hobbit:KPISeq .
